Remove RIF labels for now.

rif/abstract.v
@@ -1,7 +1,7 @@
 From mathcomp Require Import
   ssreflect ssrfun ssrbool ssrnat eqtype seq choice fintype finfun.
-From CoqUtils Require Import hseq ord fset partmap word.
-From MicroPolicies Require Import lib.utils common.types rif.common.
+From CoqUtils Require Import hseq ord partmap word.
+From MicroPolicies Require Import lib.utils common.types rif.labels.
 
 Set Implicit Arguments.
 Unset Strict Implicit.
@@ -11,157 +11,80 @@ Section Abstract.
 
 Import DoNotation.
 
-Variable Σ : finType.
+Variable L : labType.
 Variable mt : machine_types.
 Variable mops : machine_ops mt.
 Variable r_arg : reg mt.
-Variable output_addr : mword mt.
-Variable reclassify_addr : mword mt.
 
-Local Notation rifAutomaton := (rifAutomaton Σ).
-Local Notation rifLabel := (rifLabel Σ).
-Local Notation event := (event Σ mt).
-Local Notation atom := (atom (mword mt) rifLabel).
-
-Inductive ainstr : Type :=
-| ANop
-| AConst of imm mt & reg mt
-| AMov of reg mt & reg mt
-| ABinop of binop & reg mt & reg mt & reg mt
-| ALoad of reg mt & reg mt
-| AStore of reg mt & reg mt
-| AJump of reg mt
-| ABnz of reg mt & imm mt
-| AJal of reg mt & option Σ
-| AHalt.
-
-Definition ainstr_eq i1 i2 :=
-  match i1, i2 with
-  | ANop, ANop => true
-  | AConst i1 r1, AConst i2 r2 => (i1 == i2) && (r1 == r2)
-  | AMov r11 r12, AMov r21 r22 => (r11 == r21) && (r12 == r22)
-  | ABinop b1 r11 r12 r13, ABinop b2 r21 r22 r23 =>
-    [&& b1 == b2, r11 == r21, r12 == r22 & r13 == r23]
-  | ALoad r11 r12, ALoad r21 r22 => (r11 == r21) && (r12 == r22)
-  | AStore r11 r12, AStore r21 r22 => (r11 == r21) && (r12 == r22)
-  | AJump r1, AJump r2 => r1 == r2
-  | ABnz r1 i1, ABnz r2 i2 => (r1 == r2) && (i1 == i2)
-  | AJal r1 oF1, AJal r2 oF2 => (r1 == r2) && (oF1 == oF2)
-  | AHalt, AHalt => true
-  | _, _ => false
-  end.
-
-Lemma ainstr_eqP : Equality.axiom ainstr_eq.
-Proof.
-move=> i1 i2; case: i1=> *; case: i2=> * /=;
-by [
-  constructor; congruence |
-  by apply/(iffP idP)=> [/eqP ->|[->]] |
-  by apply/(iffP and4P)=> [[/eqP -> /eqP -> /eqP -> /eqP ->]|[-> -> -> ->]] |
-  by apply/(iffP andP)=> [[/eqP -> /eqP ->]|[-> ->]] ].
-Qed.
-
-Definition ainstr_eqMixin := EqMixin ainstr_eqP.
-Canonical ainstr_eqType := Eval hnf in EqType ainstr ainstr_eqMixin.
+Local Notation word := (mword mt).
+Local Notation atom := (atom word L).
 
 Record state := State {
-  mem     : {partmap mword mt -> ainstr + atom};
+  mem     : {partmap mword mt -> instr mt + atom};
   regs    : {partmap reg mt -> atom};
-  pc      : atom;
-  reclass : option Σ
+  pc      : atom
 }.
 
 Local Open Scope word_scope.
-Local Open Scope rif_scope.
+Local Open Scope label_scope.
 
 Implicit Type s : state.
 
-Definition step s : option (state * option event) :=
-  let: State mem regs pc@lpc reclass := s in
+Definition step s : option state :=
+  let: State mem regs pc@lpc := s in
   if mem pc is Some i then
     if i is inl i then
       match i with
-      | ANop => Some (State mem regs (pc + 1)@lpc None, None)
-      | AConst k r =>
-        do! regs <- updm regs r (swcast k)@⊥ₗ;
-        Some (State mem regs (pc + 1)@lpc None, None)
-      | AMov r1 r2 =>
+      | Nop => Some (State mem regs (pc + 1)@lpc)
+      | Const k r =>
+        do! regs <- updm regs r (swcast k)@⊥;
+        Some (State mem regs (pc + 1)@lpc)
+      | Mov r1 r2 =>
         do! v <- regs r1;
         do! regs <- updm regs r2 v;
-        Some (State mem regs (pc + 1)@lpc None, None)
-      | ABinop o r1 r2 r3 =>
+        Some (State mem regs (pc + 1)@lpc)
+      | Binop o r1 r2 r3 =>
         do! v1 <- regs r1;
         do! v2 <- regs r2;
-        do! regs <- updm regs r3 (binop_denote o (vala v1) (vala v2))@(taga v1 ⊔ₗ taga v2);
-        Some (State mem regs (pc + 1)@lpc None, None)
-      | ALoad r1 r2 =>
+        do! regs <- updm regs r3 (binop_denote o (vala v1) (vala v2))@(taga v1 ⊔ taga v2);
+        Some (State mem regs (pc + 1)@lpc)
+      | Load r1 r2 =>
         do! v1 <- regs r1;
         do! v2 <- mem (vala v1);
         if v2 is inr v2 then
-          do! regs <- updm regs r2 (vala v2)@(taga v1 ⊔ₗ taga v2);
-          Some (State mem regs (pc + 1)@lpc None, None)
+          do! regs <- updm regs r2 (vala v2)@(taga v1 ⊔ taga v2);
+          Some (State mem regs (pc + 1)@lpc)
         else None
-      | AStore r1 r2 =>
+      | Store r1 r2 =>
         do! v1 <- regs r1;
         do! v2 <- regs r2;
         do! vold <- mem (vala v1);
         if vold is inr vold then
-          if taga v1 ⊔ₗ lpc ⊑ₗ taga vold then
+          if taga v1 ⊔ lpc ⊑ taga vold then
             do! mem <- updm mem (vala v1)
-                                (inr (vala v2)@(taga v1 ⊔ₗ taga v2 ⊔ₗ lpc));
-            Some (State mem regs (pc + 1)@lpc None, None)
+                                (inr (vala v2)@(taga v1 ⊔ taga v2 ⊔ lpc));
+            Some (State mem regs (pc + 1)@lpc)
           else None
         else None
-      | AJump r =>
+      | Jump r =>
         do! v <- regs r;
-        Some (State mem regs (vala v)@(taga v ⊔ₗ lpc) None, None)
-      | ABnz r x =>
+        Some (State mem regs (vala v)@(taga v ⊔ lpc))
+      | Bnz r x =>
         do! v <- regs r;
         let pc' := pc + if vala v == 0 then 1
                         else swcast x in
-        Some (State mem regs pc'@(taga v ⊔ₗ lpc) None, None)
-      | AJal r oF =>
+        Some (State mem regs pc'@(taga v ⊔ lpc))
+      | Jal r =>
         do! v <- regs r;
-        do! regs <- updm regs ra (pc + 1)@(taga v ⊔ₗ lpc);
-        Some (State mem regs (vala v)@(taga v ⊔ₗ lpc) oF, None)
-      | AHalt => None
+        do! regs <- updm regs ra (pc + 1)@(taga v ⊔ lpc);
+        Some (State mem regs (vala v)@(taga v ⊔ lpc))
+      | JumpEpc => None
+      | AddRule => None
+      | GetTag _ _ => None
+      | PutTag _ _ _ => None
+      | Halt => None
       end
-    else None
-  else if pc == output_addr then
-    do! raddr <- regs ra;
-    do! out   <- regs r_arg;
-    let r_pc  := rl_readers (taga raddr) in
-    let r_out := rl_readers (taga out) in
-    Some (State mem regs raddr None,
-          Some (Output _ (vala out) (r_pc ⊔ᵣ r_out)))
-  else if pc == reclassify_addr then
-    do! raddr <- regs ra;
-    do! arg   <- regs r_arg;
-    if reclass is Some F then
-      do! regs  <- updm regs r_arg (vala arg)@(rl_trans (taga arg) F);
-      Some (State mem regs raddr None,
-            Some (Reclassify _ (taga arg) F))
     else None
   else None.
 
-Fixpoint stepn n s :=
-  if n is S n' then
-    if step s is Some (s', oe) then
-      if stepn n' s' is Some (s'', t) then
-        Some (s'', t ++ seq_of_opt oe)
-      else None
-    else None
-  else Some (s, [::]).
-
 End Abstract.
-
-Arguments ANop {Σ mt}.
-Arguments AConst {Σ mt} _ _.
-Arguments AMov {Σ mt} _ _.
-Arguments ABinop {Σ mt} _ _ _ _.
-Arguments ALoad {Σ mt} _ _.
-Arguments AStore {Σ mt} _ _.
-Arguments AJump {Σ mt} _.
-Arguments ABnz {Σ mt} _ _.
-Arguments AJal {Σ mt} _ _.
-Arguments AHalt {Σ mt}.
