rif/symbolic.v
@@ -1,7 +1,7 @@
 From mathcomp Require Import ssreflect ssrfun ssrbool ssrnat eqtype seq fintype finfun.
-From CoqUtils Require Import hseq ord fset partmap word.
+From CoqUtils Require Import hseq ord partmap word.
 From MicroPolicies
-Require Import lib.utils common.types symbolic.symbolic symbolic.exec rif.common.
+Require Import lib.utils common.types symbolic.symbolic symbolic.exec rif.labels.
 
 Set Implicit Arguments.
 Unset Strict Implicit.
@@ -11,65 +11,39 @@ Import DoNotation.
 
 Section Dev.
 
-Local Open Scope fset_scope.
-Local Open Scope rif_scope.
+Local Open Scope label_scope.
 
-Variable Σ : finType.
+Variable L : labType.
 Variable mt : machine_types.
 Variable mops : machine_ops mt.
 
-Local Notation rifAutomaton := (rifAutomaton Σ).
-Local Notation rifLabel := (rifLabel Σ).
-Local Notation event := (event Σ mt).
-
-Implicit Types r : rifAutomaton.
-
-(** Definition of tags for locations (cf. [rif_tags] below). The data
-    are tagged as follows:
-
-    - The program counter is tagged with a current label and a
-      possible reclassifier, which is only present if the last
-      executed instruction was a JAL. This is used to make sure that
-      the reclassification system service can only be invoked after a
-      JAL.
-
-    - Registers are tagged with labels, as usual.
-
-    - Memory is split among data and instructions. Instructions are
-      immutable and cannot be inspected as data. They may be tagged
-      with a reclassifier, which is only relevant when invoking the
-      reclassify system service with a JAL. Data is tagged with labels
-      as usual.
-
-    - Service entry points don't carry tags. *)
-
 Inductive mem_tag :=
-| MemInstr of option Σ
-| MemData  of rifLabel.
+| MemInstr
+| MemData of L.
 
-Definition sum_of_mem_tag t :=
+Definition option_of_mem_tag t :=
   match t with
-  | MemInstr F => inl F
-  | MemData l => inr l
+  | MemInstr => None
+  | MemData l => Some l
   end.
 
-Definition mem_tag_of_sum t :=
+Definition mem_tag_of_option t :=
   match t with
-  | inl F => MemInstr F
-  | inr l => MemData l
+  | None => MemInstr
+  | Some l => MemData l
   end.
 
-Lemma sum_of_mem_tagK : cancel sum_of_mem_tag mem_tag_of_sum.
+Lemma option_of_mem_tagK : cancel option_of_mem_tag mem_tag_of_option.
 Proof. by case. Qed.
 
-Definition mem_tag_eqMixin := CanEqMixin sum_of_mem_tagK.
+Definition mem_tag_eqMixin := CanEqMixin option_of_mem_tagK.
 Canonical mem_tag_eqType := EqType mem_tag mem_tag_eqMixin.
 
 Import Symbolic.
 
-Definition rif_tags := {|
-  pc_tag_type    := [eqType of rifLabel * option Σ];
-  reg_tag_type   := [eqType of rifLabel];
+Definition ifc_tags := {|
+  pc_tag_type    := [eqType of L];
+  reg_tag_type   := [eqType of L];
   mem_tag_type   := mem_tag_eqType;
   entry_tag_type := unit_eqType
 |}.
@@ -77,103 +51,56 @@ Definition rif_tags := {|
 (** Tag propagation rules. *)
 
 Definition instr_rules
-  (op : opcode) (tpc : rifLabel) (ti : option Σ) (ts : hseq (tag_type rif_tags) (inputs op)) :
-  option (ovec rif_tags op) :=
-  let ret := fun rtpc (rt : type_of_result rif_tags (outputs op)) => Some (@OVec rif_tags op rtpc rt) in
+  (op : opcode) (tpc : L) (ts : hseq (tag_type ifc_tags) (inputs op)) :
+  option (ovec ifc_tags op) :=
+  let ret := fun rtpc (rt : type_of_result ifc_tags (outputs op)) => Some (@OVec ifc_tags op rtpc rt) in
   match op, ts, ret with
-  | NOP, _, ret                             => ret (tpc, None) tt
-  | CONST, [hseq lold], ret                 => ret (tpc, None) ⊥ₗ
-  | MOV, [hseq l; lold], ret                => ret (tpc, None) l
-  | BINOP b, [hseq l1; l2; lold], ret       => ret (tpc, None) (l1 ⊔ₗ l2)
-  | LOAD, [hseq l1; MemData l2; lold], ret  => ret (tpc, None) (l1 ⊔ₗ l2)
-  | STORE, [hseq l1; l2; MemData lold], ret => if l1 ⊔ₗ tpc ⊑ₗ lold then
-                                                 ret (tpc, None) (MemData (l1 ⊔ₗ l2 ⊔ₗ tpc))
+  | NOP, _, ret                             => ret tpc tt
+  | CONST, [hseq lold], ret                 => ret tpc ⊥
+  | MOV, [hseq l; lold], ret                => ret tpc l
+  | BINOP b, [hseq l1; l2; lold], ret       => ret tpc (l1 ⊔ l2)
+  | LOAD, [hseq l1; MemData l2; lold], ret  => ret tpc (l1 ⊔ l2)
+  | STORE, [hseq l1; l2; MemData lold], ret => if l1 ⊔ tpc ⊑ lold then
+                                                 ret tpc (MemData (l1 ⊔ l2 ⊔ tpc))
                                                else None
-  | JUMP, [hseq l], ret                     => ret (l ⊔ₗ tpc, None) tt
-  | BNZ, [hseq l], ret                      => ret (l ⊔ₗ tpc, None) tt
-  | JAL, [hseq l1; lold], ret               => ret (l1 ⊔ₗ tpc, ti) (l1 ⊔ₗ tpc)
+  | JUMP, [hseq l], ret                     => ret (l ⊔ tpc) tt
+  | BNZ, [hseq l], ret                      => ret (l ⊔ tpc) tt
+  | JAL, [hseq l1; lold], ret               => ret (l1 ⊔ tpc) (l1 ⊔ tpc)
   | _, _, _                                 => None
   end.
 
-Definition transfer (iv : ivec rif_tags) : option (vovec rif_tags (op iv)) :=
+Definition transfer (iv : ivec ifc_tags) : option (vovec ifc_tags (op iv)) :=
   match iv with
-  | IVec (OP op) (tpc, _) ti ts =>
+  | IVec (OP op) tpc ti ts =>
     match ti with
-    | MemInstr F => @instr_rules op tpc F ts
+    | MemInstr => @instr_rules op tpc ts
     | MemData _ => None
     end
-  | IVec SERVICE (tpc, reclass) _ _ => Some tt
+  | IVec SERVICE tpc _ _ => Some tt
   end.
 
-Global Instance sym_rif : params := {
-  ttypes := rif_tags;
+Global Instance sym_ifc : params := {
+  ttypes := ifc_tags;
 
   transfer := transfer;
 
-  internal_state := [eqType of seq event]
+  internal_state := unit_eqType
 }.
 
-Local Notation state := (@Symbolic.state mt sym_rif).
+Local Notation state := (@Symbolic.state mt sym_ifc).
 
 Implicit Types st : state.
 
-Variable output_addr : mword mt.
-Variable reclassify_addr : mword mt.
-Variable r_arg : reg mt.
+Definition ifc_syscalls : syscall_table mt := emptym.
 
-Definition output_fun st : option state :=
-  do! raddr <- regs st ra;
-  do! out   <- regs st r_arg;
-  let r_pc  := rif_readers _ (rif_state (taga raddr)) in
-  let r_out := rif_readers _ (rif_state (taga out)) in
-  Some (State (mem st) (regs st) (Atom (vala raddr) (taga raddr, None))
-              (rcons (internal st) (Output _ (vala out) (r_pc ⊔ᵣ r_out)))).
-
-Definition reclassify_fun st : option state :=
-  do! raddr <- regs st ra;
-  do! arg   <- regs st r_arg;
-  if (taga (pc st)).2 is Some F then
-    do! regs  <- updm (regs st) r_arg (vala arg)@(rl_trans (taga arg) F);
-    Some (State (mem st) regs
-                (vala raddr)@(taga raddr, None)
-                (rcons (internal st) (Reclassify _ (taga arg) F)))
-  else None.
-
-Definition rif_syscalls : syscall_table mt :=
-  [partmap (output_addr, Syscall tt output_fun);
-           (reclassify_addr, Syscall tt reclassify_fun)].
-
-Local Notation step  := (@Symbolic.step mt mops sym_rif rif_syscalls).
-Local Notation ratom := (atom (mword mt) (tag_type rif_tags R)).
-Local Notation matom := (atom (mword mt) (tag_type rif_tags M)).
+Local Notation step  := (@Symbolic.step mt mops sym_ifc ifc_syscalls).
+Local Notation ratom := (atom (mword mt) (tag_type ifc_tags R)).
+Local Notation matom := (atom (mword mt) (tag_type ifc_tags M)).
 
 Hint Unfold stepf.
 Hint Unfold next_state_pc.
 Hint Unfold next_state_reg.
 Hint Unfold next_state_reg_and_pc.
 Hint Unfold next_state.
-
-Ltac step_event_app :=
-  simpl in *; repeat autounfold;
-  intros; subst; simpl in *;
-  repeat match goal with
-  | t : (_ * _)%type |- _ => destruct t; simpl in *
-  end;
-  match_inv; simpl; exists [::]; rewrite cats0.
-
-Lemma step_event_app s s' :
-  step s s' ->
-  exists t, internal s' = internal s ++ t.
-Proof.
-  case; try by step_event_app.
-  move=> /= m rs pc sc [rl oF] t -> {s} _;
-  rewrite /rif_syscalls /run_syscall mkpartmapE //=.
-  case: ifP=> [_ [<-] {sc}|_] /=.
-    rewrite /output_fun /= => e; match_inv=> /=.
-    by rewrite -cats1; eexists; eauto.
-  case: ifP=> [_ [<-] {sc}|_] //=.
-  rewrite /reclassify_fun /= => e; match_inv=> /=.
-  by rewrite -cats1; eexists; eauto.
-Qed.
 
 End Dev.
