rif/labels.v
@@ -1,0 +1,147 @@
+From mathcomp
+Require Import ssreflect ssrfun ssrbool ssrnat eqtype choice.
+
+Set Implicit Arguments.
+Unset Strict Implicit.
+Unset Printing Implicit Defensive.
+
+Delimit Scope label_scope with lab.
+
+Module Label.
+
+Section ClassDef.
+
+Record mixin_of T := Mixin {
+  join : T -> T -> T;
+  top  : T;
+  bot  : T;
+  _    : commutative join;
+  _    : associative join;
+  _    : idempotent join;
+  _    : left_id bot join;
+  _    : left_zero top join
+}.
+
+Record class_of T := Class {base : Choice.class_of T; mixin : mixin_of T}.
+Local Coercion base : class_of >->  Choice.class_of.
+
+Structure type := Pack {sort; _ : class_of sort; _ : Type}.
+Local Coercion sort : type >-> Sortclass.
+Variables (T : Type) (cT : type).
+Definition class := let: Pack _ c _ as cT' := cT return class_of cT' in c.
+Definition clone c of phant_id class c := @Pack T c T.
+Let xT := let: Pack T _ _ := cT in T.
+Notation xclass := (class : class_of xT).
+
+Definition pack m :=
+  fun b bT & phant_id (Choice.class bT) b => Pack (@Class T b m) T.
+
+(* Inheritance *)
+Definition eqType := @Equality.Pack cT xclass xT.
+
+Definition choiceType := @Choice.Pack cT xclass xT.
+
+End ClassDef.
+
+Module Import Exports.
+Coercion base : class_of >-> Choice.class_of.
+Coercion mixin : class_of >-> mixin_of.
+Coercion sort : type >-> Sortclass.
+Coercion eqType : type >-> Equality.type.
+Canonical eqType.
+Coercion choiceType : type >-> Choice.type.
+Canonical choiceType.
+Notation labType := type.
+Notation labMixin := mixin_of.
+Notation LabMixin := Mixin.
+Notation LabType T m := (@pack T m _ _ id).
+Notation "[ 'labType' 'of' T 'for' cT ]" :=  (@clone T cT _ idfun)
+  (at level 0, format "[ 'labType'  'of'  T  'for'  cT ]") : form_scope.
+Notation "[ 'labType' 'of' T ]" := (@clone T _ _ id)
+  (at level 0, format "[ 'labType'  'of'  T ]") : form_scope.
+End Exports.
+
+End Label.
+
+Export Label.Exports.
+
+Section Theory.
+
+Local Open Scope label_scope.
+
+Variable L : labType.
+
+Implicit Types (l : L).
+
+Definition join := Label.join (Label.class L).
+Definition top := Label.top (Label.class L).
+Definition bot := Label.bot (Label.class L).
+
+Local Notation "l1 ⊔ l2" :=
+  (join l1 l2) (at level 40, left associativity) : label_scope.
+Local Notation "⊤" := top : label_scope.
+Local Notation "⊥" := bot : label_scope.
+
+Lemma joinC : commutative join.
+Proof. by rewrite /join; case: (L)=> [? [? []]]. Qed.
+
+Lemma joinA : associative join.
+Proof. by rewrite /join; case: (L)=> [? [? []]]. Qed.
+
+Lemma joinll : idempotent join.
+Proof. by rewrite /join; case: (L)=> [? [? []]]. Qed.
+
+Lemma joinBl : left_id ⊥ join.
+Proof. by rewrite /bot /join; case: (L)=> [? [? []]]. Qed.
+
+Lemma joinTl : left_zero ⊤ join.
+Proof. by rewrite /top /join; case: (L)=> [? [? []]]. Qed.
+
+Lemma joinlB : right_id ⊥ join.
+Proof. by move=> l; rewrite joinC joinBl. Qed.
+
+Lemma joinlT : right_zero ⊤ join.
+Proof. by move=> l; rewrite joinC joinTl. Qed.
+
+(* XXX: Should this be a notation? *)
+Definition flows l1 l2 := l1 ⊔ l2 == l2.
+
+Local Notation "l1 ⊑ l2" :=
+  (flows l1 l2) (at level 50, no associativity) : label_scope.
+
+Lemma flowsll : reflexive flows.
+Proof. by move=> l; rewrite /flows joinll eqxx. Qed.
+
+Lemma flows_trans : transitive flows.
+Proof.
+by move=> ???; rewrite /flows => /eqP e /eqP <-; rewrite joinA e.
+Qed.
+
+Lemma flows_antisym : antisymmetric flows.
+Proof.
+move=> l l'; rewrite /flows => /andP [/eqP e1 /eqP e2].
+by rewrite -e2 joinC.
+Qed.
+
+Lemma flows_join l l1 l2 : (l1 ⊔ l2 ⊑ l) = (l1 ⊑ l) && (l2 ⊑ l).
+Proof.
+rewrite /flows; apply/(sameP idP)/(iffP andP).
+  by case=> [e1 /eqP e2]; rewrite -joinA e2.
+move=> /eqP e; rewrite -{}e 2!joinA joinll; split=> //.
+by rewrite 2!joinA [l2 ⊔ _]joinC -3!joinA [l2 ⊔ _]joinA joinll.
+Qed.
+
+Lemma botP l : ⊥ ⊑ l.
+Proof. by rewrite /flows joinBl. Qed.
+
+Lemma topP l : l ⊑ ⊤.
+Proof. by rewrite /flows joinlT. Qed.
+
+End Theory.
+
+Notation "l1 ⊔ l2" :=
+  (join l1 l2) (at level 40, left associativity) : label_scope.
+Notation "⊤" := (top _) : label_scope.
+Notation "⊥" := (bot _) : label_scope.
+Notation "l1 ⊑ l2" :=
+  (flows l1 l2) (at level 50, no associativity) : label_scope.
